Further progress on new linking simulation proof

sepcomp/linking_sim.v
@@ -66,9 +66,20 @@ Defined.
 
 Lemma types_eq {c : Core.t cores_S} {d : Core.t cores_T} (pf : c.(Core.i)=d.(Core.i)) : 
   C (cores_T (Core.i d))=C (cores_T (Core.i c)).
-Proof. by rewrite pf. Qed.
+Proof. by rewrite pf. Defined.
+
+Lemma types_eq' {c : Core.t cores_S} {d : Core.t cores_T} (pf : c.(Core.i)=d.(Core.i)) : 
+  C (cores_T (Core.i c))=C (cores_T (Core.i d)).
+Proof. by rewrite pf. Defined.
 
 Notation cast pf x := (cast_ty (types_eq pf) x).
+
+Notation cast' pf x := (cast_ty (types_eq' pf) x).
+
+Lemma cast_cast'_eq 
+  {c : Core.t cores_S} {d : Core.t cores_T} (pf : c.(Core.i)=d.(Core.i)) 
+  (x : C (cores_T c.(Core.i))) : cast pf (cast' pf x) = x.
+Proof. Admitted. (* TODO *)
 
 Section frame_inv.
 
@@ -79,16 +90,56 @@ Variable  pf : c.(i)=d.(i).
 
 Require Import compcert.lib.Coqlib. (*for Forall2*)
 
+(** Frame Invariant: 
+    ~~~~~~~~~~~~~~~~
+
+   The frame invariant applies to cores in caller positions in the
+   call stack.  I.e, to cores that are waiting [at_external] for the
+   environment to return. Main arguments are:
+
+   * Existentially quantified when [frame_inv] is applied:
+   -[mu0]: [SM_injection] at point of external call
+
+   -[nu0]: [SM_injection] derived from [mu0] by restricting [pubSrc]
+   and [pubTgt] to reachable local blocks.  [nu0] is used primarily to
+   state the [unchOn] invariants assumable by THIS core.
+
+   -[m10], [m20]: Source and target memories active at call point. 
+
+   * True parameters: 
+   -[mu]: The [SM_injection] of the currently running core (/not/ this
+    one).  Things to note:
+
+     +When we resume a core, we do not use [mu] directly.  Instead, we
+     employ the derived [SM_injection]:
+
+       nu := { local_of  := local_of nu0
+             ; extern_of := extern_of nu0 
+                            + {extern_of mu | REACH m1' m2' ret1 ret2}
+             ; ... }
+
+     This [SM_injection] satisfies [extern_incr nu0 nu], among other
+     properties required by the [after_external] clause of structured
+     simulations.
+
+   -[m1], [m2]: Active memories. 
+*)
+
 Record frame_inv cd0 mu0 mu m10 m1 e1 ef_sig1 vals1 m20 m2 e2 ef_sig2 vals2 : Type :=
   { (* local definitions *)
-    pubSrc' := fun b => [&& locBlocksSrc mu0 b & REACH m10 (exportedSrc mu0 vals1) b] 
-  ; pubTgt' := fun b => [&& locBlocksTgt mu0 b & REACH m20 (exportedTgt mu0 vals2) b] 
-  ; nu0     := replace_locals mu0 pubSrc' pubTgt'
+    pubSrc := fun b => [&& locBlocksSrc mu0 b & REACH m10 (exportedSrc mu0 vals1) b] 
+  ; pubTgt := fun b => [&& locBlocksTgt mu0 b & REACH m20 (exportedTgt mu0 vals2) b] 
+  ; nu0    := replace_locals mu0 pubSrc pubTgt
 
     (* invariants required to instantiate at_external *)
-  ; frame_inj   : Mem.inject (as_inj mu0) m10 m20
-  ; frame_match : (sims c.(i)).(match_state) cd0 mu0 c.(Core.c) m10 (cast pf d.(Core.c)) m20 
-  ; frame_at1   : at_external (cores_S c.(i)).(coreSem) c.(Core.c) = Some (e1, ef_sig1, vals1) 
+  ; frame_inj0  : Mem.inject (as_inj mu0) m10 m20
+  ; frame_inj   : Mem.inject (as_inj mu0) m1 m2
+
+  ; frame_match : (sims c.(i)).(match_state) cd0 mu0 
+                    c.(Core.c) m10 (cast pf d.(Core.c)) m20 
+
+  ; frame_at1   : at_external (cores_S c.(i)).(coreSem) c.(Core.c) 
+                    = Some (e1, ef_sig1, vals1) 
   ; frame_at2   : at_external (cores_T c.(i)).(coreSem) (cast pf d.(Core.c)) 
                     = Some (e2, ef_sig2, vals2) 
   ; frame_vinj  : Forall2 (val_inject (as_inj mu0)) vals1 vals2  
@@ -96,13 +147,36 @@ Record frame_inv cd0 mu0 mu m10 m1 e1 ef_sig1 vals1 m20 m2 e2 ef_sig2 vals2 : Ty
   ; frame_fwd1  : mem_forward m10 m1
   ; frame_fwd2  : mem_forward m20 m2
 
-  ; frame_unch1 : Mem.unchanged_on [fun b ofs => [/\ locBlocksSrc nu0 b & pubBlocksSrc nu0 b]] m10 m1
+  ; frame_unch1 : Mem.unchanged_on [fun b ofs => 
+                    [/\ locBlocksSrc nu0 b & pubBlocksSrc nu0 b=false]] m10 m1
   ; frame_unch2 : Mem.unchanged_on (local_out_of_reach nu0 m10) m20 m2 
 
-  ; frame_incr : StructuredInjections.intern_incr mu0 mu
-  ; frame_sep  : StructuredInjections.sm_inject_separated mu0 mu m10 m20 }.
+  ; frame_sep  : StructuredInjections.sm_inject_separated nu0 mu m10 m20 }.
 
 End frame_inv.
+
+(** These lemmas on [restrict_sm] should go elsewhere. *)
+
+Lemma restrict_some {mu b1 b2 d X} : 
+  (restrict mu X) b1 = Some (b2, d) -> mu b1 = Some (b2, d).
+Proof. by rewrite/restrict; case: (X b1). Qed.
+
+Lemma restrict_sm_domsrc {mu b1 X} : DomSrc (restrict_sm mu X) b1 -> DomSrc mu b1.
+Proof. by rewrite/restrict_sm; case: mu. Qed.
+
+Lemma restrict_sm_domtgt {mu b2 X} : DomTgt (restrict_sm mu X) b2 -> DomTgt mu b2.
+Proof. by rewrite/restrict_sm; case: mu. Qed.
+
+Lemma sm_inject_separated_restrict mu mu' m1 m2 X : 
+  sm_inject_separated mu mu' m1 m2 -> 
+  sm_inject_separated mu (restrict_sm mu' X) m1 m2.
+Proof.
+move=>[]H []H2 H3; split.
+move=> b1 b2 d A; rewrite restrict_sm_all; move/restrict_some=> B.
+by apply: (H _ _ _ A B).
+split; first by move=> b1 A; move/restrict_sm_domsrc=> B; apply: (H2 _ A B).
+by move=> b2 A; move/restrict_sm_domtgt=> B; apply: (H3 _ A B).
+Qed.
 
 Section head_inv.
 
@@ -112,7 +186,8 @@ Variables (c : t cores_S) (d : t cores_T).
 Variable  (pf : c.(i)=d.(i)).
 
 Record head_inv cd mu m1 m2 : Type :=
-  { head_match : (sims c.(i)).(match_state) cd mu c.(Core.c) m1 (cast pf d.(Core.c)) m2 }.
+  { head_match : (sims c.(i)).(match_state) cd mu 
+                   c.(Core.c) m1 (cast pf d.(Core.c)) m2 }.
 
 End head_inv.
 
@@ -131,7 +206,8 @@ Qed.
 
 End head_inv_lems.
 
-Fixpoint tail_inv mu (s1 : Stack.t (Core.t cores_S)) (s2 : Stack.t (Core.t cores_T)) m1 m2 :=
+Fixpoint tail_inv mu 
+  (s1 : Stack.t (Core.t cores_S)) (s2 : Stack.t (Core.t cores_T)) m1 m2 :=
   match s1, s2 with
     | c :: s1', d :: s2' => 
       [/\ exists (pf : c.(Core.i)=d.(Core.i)) cd0 mu0,
@@ -157,14 +233,15 @@ Lemma tail_inv_restrict (X : block -> bool) :
   REACH_closed m1 X -> 
   tail_inv (restrict_sm mu X) s1 s2 m1 m2.
 Proof.
-move=> H H2; move: s2 tail_len_eq inv.
-elim: s1=> // a s1' IH s0; case: s0=> // b s2' H3.
+move=> H H2; move: s2 tail_len_eq inv; elim: s1=> // a s1' IH s0. 
+case: s0=> // b s2' H3.
 have H4: length s1' = length s2' by move: H3=> /=; case.
 move=> /= [] H5; split; last by apply: IH.
 move: H5=> [pf][cd][mu0][m10][e1][sig1][vals1][m20][e2][sig2][vals2][].
-exists pf, cd, (restrict_sm mu0 X), m10, e1, sig1, vals1, m20, e2, sig2, vals2.
+exists pf, cd, mu0, m10, e1, sig1, vals1, m20, e2, sig2, vals2. 
 apply: Build_frame_inv=> //.
-Admitted. (*TODO*)
+by apply: sm_inject_separated_restrict.
+Qed.
 
 End tail_inv_lems.
 
@@ -183,7 +260,7 @@ Record R (data : Lex.t types) mu (x1 : linker N cores_S) m1 (x2 : linker N cores
   ; d   := stack.head _ pf2 
     (* invariants *)
   ; R_head : exists (pf : c.(Core.i)=d.(Core.i)) cd, head_inv c d pf cd mu m1 m2 
-  ; R_tail : tail_inv mu s1.(callStack) s2.(callStack) m1 m2 }.
+  ; R_tail : tail_inv mu (pop s1.(callStack)) (pop s2.(callStack)) m1 m2 }.
 
 End R.
 
@@ -193,6 +270,43 @@ Context data mu x1 m1 x2 m2 (pf : R data mu x1 m1 x2 m2).
 
 Import CallStack.
 Import Linker.
+
+Lemma peekpeek_match c1 c2 (pf0 : Core.i c1=Core.i c2) : 
+  peekCore x1 = Some c1 -> 
+  peekCore x2 = Some c2 -> 
+  exists cd, 
+  match_state (sims (Core.i c1)) cd mu (Core.c c1) m1 (cast pf0 (Core.c c2)) m2.
+Proof.
+move: (R_head pf)=> [A][B]; move/head_match=> MATCH H1 H2.
+move: A B MATCH; rewrite/c/d/s1/s2/stack.head.
+rewrite (StackDefs.peeksome_head _ H1 (pf1 pf)). 
+rewrite (StackDefs.peeksome_head _ H2 (pf2 pf)).
+move=> A cd MATCH; exists cd. 
+have ->: (cast pf0 (Core.c c2) = cast A (Core.c c2)).
+  by f_equal; f_equal; apply proof_irr.
+by [].
+Qed.
+
+Lemma peek_peek c1 : 
+  peekCore x1 = Some c1 -> 
+  exists c2, Core.i c1=Core.i c2 /\ peekCore x2 = Some c2.
+Proof.
+move: (R_head pf)=> [A][B]; move/head_match=> MATCH H.
+have ->: (c1 = c pf) by rewrite/c/stack.head (StackDefs.peeksome_head _ H (pf1 pf)).
+exists (d pf); split=> //.
+rewrite/peekCore/peek StackDefs.nonempty_peek; first by apply: (pf2 pf).
+by move=> C; rewrite/d/stack.head/s2; f_equal; f_equal; apply: proof_irr.
+Qed.
+
+Lemma peek_peekmatch c1 : 
+  peekCore x1 = Some c1 -> 
+  exists c2 (pf0: Core.i c1=Core.i c2) cd,
+  peekCore x2 = Some c2
+  /\ match_state (sims (Core.i c1)) cd mu (Core.c c1) m1 (cast pf0 (Core.c c2)) m2.
+Proof.
+move=> H1; move: (peek_peek H1)=> []c2 []pf0 H2. 
+by move: (peekpeek_match pf0 H1 H2)=> []cd MATCH; exists c2, pf0, cd; split.
+Qed.
 
 Lemma R_wd : SM_wd mu.
 Proof. 
@@ -230,7 +344,8 @@ Lemma R_match_restrict (X : block -> bool) :
   R data (restrict_sm mu X) x1 m1 x2 m2.
 Proof.
 move: (R_head pf)=> [A][B]; move/head_inv_restrict=> H H2 H3; move: (H _ H2 H3)=> H'.
-admit. (*by tail_inv_restrict*)
+apply: Build_R; first by exists A, B; apply: H'. 
+by apply: tail_inv_restrict=> //; apply: (R_tail pf). 
 Qed.
 
 Lemma R_match_validblocks : sm_valid mu m1 m2.
@@ -278,8 +393,68 @@ eapply Build_SM_simulation_inject
 - by admit.
 
 (* real diagram *)
-- admit. 
+- move=> st1 m1 st1' m1' U1 STEP data st2 mu m2 U1_DEF INV.
+case: STEP=> STEP STEP_EFFSTEP.
+case: STEP.
+ (* Case: corestep0 *)
+ + move=> STEP. 
 
+ have [c1 A]: exists c, peekCore st1 = Some c. 
+  { by move: STEP; rewrite/Sem.corestep0; case: (peekCore st1)=> // a; exists a. }
+
+ have [c1' [STEP0 ST1']]: 
+         exists c' : C (cores_S (Core.i c1)), 
+         Coresem.corestep (t := Effectsem.instance (coreSem (cores_S (Core.i c1)))) 
+            (ge (cores_S (Core.i c1))) (Core.c c1) m1 c' m1' 
+         /\ st1' = updCore st1 (Core.upd c1 c').
+  { by move: STEP; rewrite/Sem.corestep0 A=> [][]c' []B C; exists c'; split. }
+
+ have EFFSTEP: 
+        effect_semantics.effstep (coreSem (cores_S (Core.i c1))) 
+        (ge (cores_S (Core.i c1))) U1 (Core.c c1) m1 c1' m1'.
+  { move: (STEP_EFFSTEP STEP); rewrite/effstep0 A=> [][] c1'' [] STEP0' ST1''.
+    by rewrite ST1'' in ST1'; rewrite -(updCore_inj_upd ST1'). }
+
+ (* specialize core diagram at module (Core.i c1) *)
+ move: (effcore_diagram_strong_perm _ _ _ _ _ (sims (Core.i c1))).  
+ move/(_ _ _ _ _ _ EFFSTEP).
+ move/(_ _ _ _ _ U1_DEF).
+ move: (peek_peekmatch INV A)=> []c2 []pf0 []cd []B MATCH.
+ move/(_ _ _ _ MATCH).
+
+ move=> []c2' []m2' []cd' []mu'.
+ move=> []INCR []SEP []LOCALLOC []MATCH' []U2 []STEP' PERM.
+
+ (* instantiate existentials *)
+ set c2''  := cast' pf0 c2'.
+ set st2'  := updCore st2 (Core.upd c2 c2'').
+ set data' := Lex.set (Core.i c1) cd' data.
+
+ exists st2', m2', data', mu'.
+ split=> //.
+ split=> //.
+ split=> //.
+ split. 
+
+ (* re-establish invariant *)
+ have A' : peekCore st1' = Some (Core.upd c1 c1') by rewrite ST1'.
+ have B' : peekCore st2' = Some (Core.upd c2 c2'') by rewrite/st2'.
+ rewrite/peekCore in A' B'.
+
+ apply: Build_R; rewrite/stack.head. 
+ rewrite (StackDefs.peeksome_head _ A') (StackDefs.peeksome_head _ B')=> /=. 
+
+ (* head_inv *)
+ + { exists pf0, cd'; apply: Build_head_inv=> /=.
+     by rewrite /c2''; rewrite cast_cast'_eq; apply: MATCH'. }
+
+ (* tail_inv *)
+ + { admit. (* TODO *)}
+
+ exists U2.
+ split=> //.
+ case: STEP'=> STEP'. left. admit. (* TODO: -->+  implies  ==>+ *)
+ 
 Admitted. (*WORK-IN-PROGRESS*)
 
 End linkingSimulation.
