sepcomp/stack.v
@@ -20,9 +20,8 @@ Definition empty : Stack.t T := [::].
 Definition nonempty : pred (Stack.t T) := 
   [pred s | if s is [::] then false else true].
 
-Lemma peek_nonempty (stack : Stack.t T) : 
-  nonempty stack -> exists t, peek stack = Some t.
-Proof. by case: stack=>// a l _; exists a. Qed.
+Lemma peek_nonempty (stack : Stack.t T) t : peek stack = Some t -> nonempty stack.
+Proof. by rewrite/peek; case: stack. Qed.
 
 Lemma nonempty_nempty (stack: Stack.t T) : nonempty stack -> [::] = stack -> T.
 Proof. by case: stack. Qed.
@@ -32,6 +31,15 @@ Definition head (stack: Stack.t T) (pf: nonempty stack) : T :=
     | nil => fun pf' => nonempty_nempty pf pf'
     | s :: stack' => fun pf' => s
   end) erefl.
+
+Lemma nonempty_peek (stack : Stack.t T) (pf : nonempty stack) : 
+  peek stack = Some (head stack pf).
+Proof. by move: pf; case: stack=>// a l _. Qed.
+
+Lemma peeksome_head stack t : 
+  peek stack = Some t -> 
+  forall pf : nonempty stack, head stack pf = t.
+Proof. by rewrite/head; case: stack=> //=; move=> ? ?; case. Qed.
 
 Lemma all_pop (stack : Stack.t T) p : all p stack -> all p (pop stack).
 Proof. by case: stack=>//= a l; move/andP=> [H1 H2]. Qed.
